separate for loop share and each packet

src/mqtt-packet-parser/src/common.fst
@@ -8,6 +8,7 @@ module HS = FStar.HyperStack
 open FStar.HyperStack.ST
 open LowStar.BufferOps
 open FStar.Int.Cast
+open LowStar.Printf
 open C.String
 
 
@@ -80,6 +81,85 @@ let decodeing_variable_bytes ptr_for_decoding_packets bytes_length =
     ptr_for_remaining_length.(0ul) in
   pop_frame ();
   remaining_length
+
+
+val get_variable_byte: packet_data: (B.buffer U8.t) 
+  -> packet_size: type_packet_size 
+  -> now_index:U32.t
+  -> Stack (variable_length: struct_variable_length)
+    (requires fun h0 -> B.live h0 packet_data)
+    (ensures fun h0 r h1 -> true)
+let get_variable_byte packet_data packet_size now_index =
+  push_frame ();
+  let ptr_for_decoding_packets: B.buffer U8.t = B.alloca 0uy 4ul in
+  let ptr_remaining_length: B.buffer type_remaining_length =
+   B.alloca 0ul 1ul in
+  let ptr_byte_length: B.buffer U8.t = B.alloca 0uy 1ul in
+  let ptr_next_start_index: B.buffer U32.t = B.alloca 0ul 1ul in
+  let loop_last: U32.t = 
+    (
+      if U32.( (packet_size -^ now_index ) <^ 4ul) then
+        packet_size 
+      else
+        U32.add now_index 4ul
+    ) in
+  let inv h (i: nat) = B.live h packet_data /\ 
+  B.live h ptr_for_decoding_packets /\
+  B.live h ptr_remaining_length /\
+  B.live h ptr_byte_length in
+  let body (i): Stack unit
+    (requires (fun h -> inv h (U32.v i)))
+    (ensures (fun _ _ _ -> true)) =
+      if (ptr_byte_length.(0ul) = 0uy) then
+        (
+          let j = U32.sub i now_index in
+          ptr_for_decoding_packets.(j) <- packet_data.(i);
+          let is_end_byte: bool =
+            (
+              if (U32.eq i 1ul && U8.lte packet_data.(i) 0x7Fuy) ||
+                (U32.gte i 2ul && U8.gte packet_data.(i) 0x01uy && U8.lte packet_data.(i) 0x7Fuy)
+                then
+                true
+              else
+                false
+            ) in
+
+            if (is_end_byte) then
+              (
+                let bytes_length_u8: U8.t = uint32_to_uint8(U32.add j 1ul) in
+                let untrust_remaining_length: type_remaining_length =
+                  decodeing_variable_bytes ptr_for_decoding_packets bytes_length_u8 in
+                let byte_length: U32.t = U32.add untrust_remaining_length i in
+                let valid_remaining_length: bool = 
+                  U32.eq (U32.sub packet_size 1ul) (U32.add untrust_remaining_length i) in
+                if valid_remaining_length then (
+                  ptr_remaining_length.(0ul) <- untrust_remaining_length;
+                  ptr_byte_length.(0ul) <- bytes_length_u8;
+                  ptr_next_start_index.(0ul) <- U32.add i 1ul
+                )           
+              )
+        )
+  in
+  C.Loops.for now_index loop_last inv body;
+  let remaining_length = ptr_remaining_length.(0ul) in
+  let byte_length = ptr_byte_length.(0ul) in
+  let next_start_index = ptr_next_start_index.(0ul) in
+  pop_frame ();
+
+  print_u8 byte_length;
+  print_string "\n";
+  if (byte_length = 0uy) then
+    {
+      have_error = true;
+      variable_length_value = max_u32;
+      next_start_index = max_u32;
+    }
+  else
+    {
+      have_error = false;
+      variable_length_value = remaining_length;
+      next_start_index = next_start_index;
+    }
 
 val get_message_type: message_type_bits: U8.t -> type_mqtt_control_packets_restrict
 let get_message_type message_type_bits =
